concurrency/scache/ClientCounter.i.dfy
@@ -1,6 +1,109 @@
-module ClientCounter {
-  type Client
+include "../framework/BasicPCM.i.dfy"
 
-  glinear method hack_new_client()
-  returns (glinear client: Client)
+module CounterPCM refines BasicPCM {
+  ghost const max: nat := 0xff
+
+  datatype M = Counter(n: nat)
+
+  function dot(x: M, y: M) : M
+  {
+    Counter(x.n + y.n)
+  }
+
+  predicate valid(x: M) 
+  {
+    x.n <= max
+  }
+
+  function unit() : M
+  {
+    Counter(0)
+  }
+
+  lemma dot_unit(x: M)
+  ensures dot(x, unit()) == x
+  {
+  }
+
+  lemma valid_unit(x: M)
+  ensures valid(unit())
+  {
+  }
+
+  lemma commutative(x: M, y: M)
+  ensures dot(x, y) == dot(y, x)
+  {
+  }
+
+  lemma associative(x: M, y: M, z: M)
+  ensures dot(x, dot(y, z)) == dot(dot(x, y), z)
+  {
+  }
+}
+
+module ClientCounter {
+  import T = Tokens(CounterPCM)
+  import opened GhostLoc
+  import opened CounterPCM
+
+  datatype {:glinear_fold} Client = Client(ghost loc: Loc)
+  {
+    function defn() : T.Token {
+      T.Token(loc, Counter(1))
+    }
+  }
+
+  datatype {:glinear_fold} Clients = Clients(ghost loc: Loc, ghost n: nat)
+  {
+    function defn() : T.Token {
+      T.Token(loc, Counter(n))
+    }
+  }
+
+  glinear method counter_init()
+  returns (glinear cl: Clients)
+  ensures cl.n == max
+  {
+    glinear var t := T.init(Counter(max));
+    cl := Clients_fold(Clients(t.loc, max), t);
+  }
+
+  glinear method get_bound(gshared cs: Clients)
+  ensures cs.n <= max
+  {
+    gshared var s := Clients_unfold_borrow(cs);
+    glinear var u := T.get_unit(cs.loc);
+    T.is_valid(s, inout u);
+    T.dispose(u);
+  }
+
+  glinear method merge(glinear cs: Clients, glinear c: Client)
+  returns (glinear cs': Clients)
+  requires cs.loc == c.loc
+  ensures cs' == Clients(cs.loc, cs.n + 1)
+  {
+    glinear var a := Clients_unfold(cs);
+    glinear var b := Client_unfold(c);
+    glinear var x := T.join(a, b);
+    cs' := Clients_fold(Clients(cs.loc, cs.n + 1), x);
+  }
+
+  glinear method split(glinear cs: Clients)
+  returns (glinear cs': Clients, glinear c': Client)
+  requires cs.n >= 1
+  ensures cs' == Clients(cs.loc, cs.n - 1)
+  ensures c' == Client(cs.loc)
+  {
+    glinear var a := Clients_unfold(cs);
+    glinear var x, y := T.split(a,
+        Counter(cs.n - 1),
+        Counter(1));
+    cs' := Clients_fold(Clients(cs.loc, cs.n - 1), x);
+    c' := Client_fold(Client(cs.loc), y);
+  }
+
+  glinear method empty_counter(ghost loc: Loc)
+  returns (glinear cs': Clients)
+  ensures cs'.n == 0
+  ensures cs'.loc == loc
 }
