concurrency/framework/BasicPCM.i.dfy
@@ -1,0 +1,25 @@
+include "PCM.s.dfy"
+
+abstract module BasicPCM refines PCM {
+  predicate transition(a: M, b: M) {
+    forall c :: valid(dot(a, c)) ==> valid(dot(b, c))
+  }
+  
+  lemma transition_is_refl(a: M)
+  {
+  }
+
+  lemma transition_is_trans(a: M, b: M, c: M)
+  {
+  }
+
+  lemma transition_is_monotonic(a: M, b: M, c: M)
+  {
+    forall d | valid(dot(dot(a, c), d))
+    ensures valid(dot(dot(b, c), d))
+    {
+      associative(a, c, d);
+      associative(b, c, d);
+    }
+  }
+}
